src/Bedrock/Proofs/ValidComputable/Expr.v
@@ -6,7 +6,7 @@ Require Import bedrock2.Syntax.
 Require Import coqutil.Word.Interface coqutil.Word.Properties.
 Require Import coqutil.Map.Interface.
 Require Import Crypto.Bedrock.Types.
-Require Import Crypto.Bedrock.Translation.Expr.
+Require Import Crypto.Bedrock.Field.Translation.Expr.
 Require Import Crypto.Bedrock.Proofs.Expr.
 Require Import Crypto.Language.API.
 Require Import Crypto.Util.Decidable.
