src/Bedrock/Synthesis/Examples/EncodeDecode.v
@@ -13,9 +13,9 @@ Require Import Crypto.Arithmetic.Partition.
 Require Import Crypto.Bedrock.Parameters.Defaults.
 Require Import Crypto.Bedrock.Tactics.
 Require Import Crypto.Bedrock.Types.
-Require Import Crypto.Bedrock.Field.Bignum.
-Require Import Crypto.Bedrock.Field.Operation.
-Require Import Crypto.Bedrock.Field.UnsaturatedSolinas.
+Require Import Crypto.Bedrock.Field.Generic.Bignum.
+Require Import Crypto.Bedrock.Field.Generic.Operation.
+Require Import Crypto.Bedrock.Field.Generic.UnsaturatedSolinas.
 Require Import Crypto.Bedrock.Synthesis.Tactics.
 Require Import Crypto.Bedrock.Synthesis.UnsaturatedSolinas.
 Require Import Crypto.Bedrock.Synthesis.Examples.X25519_64.
